Add atom swap support for choice types

ChoiceType/theories/Qualifier.v
@@ -39,6 +39,13 @@ Definition qual_open_atom (k : nat) (x : atom) (q : type_qualifier) : type_quali
       else q
   end.
 
+Definition qual_swap_atom (x y : atom) (q : type_qualifier) : type_qualifier :=
+  match q with
+  | qual B d p =>
+      qual B (aset_swap x y d)
+        (λ β σ a, p β (store_swap x y σ) (store_swap x y a))
+  end.
+
 Definition qual_and (q1 q2 : type_qualifier) : type_qualifier :=
   match q1, q2 with
   | qual B1 d1 p1, qual B2 d2 p2 =>
@@ -78,6 +85,7 @@ Arguments stale_qualifier /.
 Arguments open_qual_atom_inst /.
 
 Notation "q '^q^' x" := (qual_open_atom 0 x q) (at level 20).
+Notation "q '^qs^' '(' x ',' y ')'" := (qual_swap_atom x y q) (at level 20).
 
 (** ** Local closure *)
 
