ChoiceType/theories/LocallyNamelessProps.v
@@ -12,3 +12,42 @@
 From LocallyNameless Require Import Classes.
 From ChoiceType Require Export Syntax QualifierProps.
 From ChoiceType Require Import QualifierInstances.
+
+(** ** Atom swap facts *)
+
+Lemma cty_fv_swap x y τ :
+  fv_cty (cty_swap_atom x y τ) = aset_swap x y (fv_cty τ).
+Proof.
+  induction τ; simpl; try rewrite ?qual_dom_swap;
+    try rewrite ?IHτ1, ?IHτ2, <- ?aset_swap_union; reflexivity.
+Qed.
+
+Lemma ctx_fv_swap x y Γ :
+  ctx_fv (ctx_swap_atom x y Γ) = aset_swap x y (ctx_fv Γ).
+Proof.
+  induction Γ; simpl.
+  - symmetry. apply aset_swap_empty.
+  - rewrite cty_fv_swap.
+    rewrite <- aset_swap_singleton, <- aset_swap_union.
+    reflexivity.
+  - rewrite IHΓ1, IHΓ2, <- aset_swap_union. reflexivity.
+  - rewrite IHΓ1, IHΓ2, <- aset_swap_union. reflexivity.
+  - rewrite IHΓ1, IHΓ2, <- aset_swap_union. reflexivity.
+Qed.
+
+Lemma ctx_dom_swap x y Γ :
+  ctx_dom (ctx_swap_atom x y Γ) = aset_swap x y (ctx_dom Γ).
+Proof.
+  induction Γ; simpl.
+  - symmetry. apply aset_swap_empty.
+  - rewrite <- aset_swap_singleton. reflexivity.
+  - rewrite IHΓ1, IHΓ2, <- aset_swap_union. reflexivity.
+  - rewrite IHΓ1, IHΓ2, <- aset_swap_union. reflexivity.
+  - rewrite IHΓ1, IHΓ2, <- aset_swap_union. reflexivity.
+Qed.
+
+Lemma cty_swap_preserves_erasure x y τ :
+  erase_ty (cty_swap_atom x y τ) = erase_ty τ.
+Proof.
+  induction τ; simpl; congruence.
+Qed.
